fixing stuff on Imp

theories/Relational/Imp.v
@@ -64,11 +64,11 @@ Section ImpMonad.
 
   Eval cbv in W ⟨one,one⟩.
 
-  Definition Wun := STCont S.
+  Definition Wun := STCont (S × S).
 
   Eval cbv in (Wun bool).
 
-  Let R := (@omon_rel Wun).
+  Let R (A : Type) := (@omon_rel Wun A).
 
   Program Definition ffixun {A} (f : Wun A -> Wun A) : Wun A := ⦑fun post s0 => forall w, R (f w) w -> Spr1 w post s0 ⦒.
   Next Obligation.
@@ -78,23 +78,47 @@ Section ImpMonad.
 
   Eval cbv in (Wun bool).
 
-  Program Definition Wunget {A : Type} (k : S -> Wun A) : Wun A := ⦑fun post s0 => Spr1 (k s0) post s0⦒.
-  Next Obligation. cbv.  intros x y H s H'. destruct (k s). cbv in Spr2.  apply (Spr2 x y); intuition. Qed.
+  Program Definition WungetL {A : Type} (k : S -> Wun A) : Wun A := ⦑fun post s0 => Spr1 (k (nfst s0)) post s0⦒.
+  Next Obligation. cbv. intros x y H [sl sr] H'.
+                   destruct (k sl). cbv in Spr2. apply (Spr2 x y); intuition.
+  Qed.
 
-  Program Definition Wunset {A : Type} (s : S) (k : Wun A) : Wun A := ⦑fun post _ => Spr1 k post s⦒.
+  Program Definition WungetR {A : Type} (k : S -> Wun A) : Wun A := ⦑fun post s0 => Spr1 (k (nsnd s0)) post s0⦒.
+  Next Obligation. cbv.  intros x y H [sl sr] H'. destruct (k sr). cbv in Spr2.  apply (Spr2 x y); intuition. Qed.
+
+  Program Definition WunsetL {A : Type} (s : S) (k : Wun A) : Wun A := ⦑fun post s0 => Spr1 k post (npair s (nsnd s0))⦒.
+  Next Obligation. cbv. intros x y H s0 H''. destruct k. cbv in Spr2. apply (Spr2 x y); intuition.  Qed.
+  Program Definition WunsetR {A : Type} (s : S) (k : Wun A) : Wun A := ⦑fun post s0 => Spr1 k post (npair (nfst s0) s)⦒.
   Next Obligation. cbv. intros x y H s0 H''. destruct k. cbv in Spr2. apply (Spr2 x y); intuition.  Qed.
 
-  Fixpoint θun (A : Type) (c: Imp A) {struct c} : Wun A :=
+  Fixpoint θunL (A : Type) (c: Imp A) {struct c} : Wun A :=
       match c with
       | ImpRet a => @ret Wun _ a
-      | ImpGet k => Wunget (fun s => θun (k s))
-      | ImpSet s k => Wunset s (θun k)
+      | ImpGet k => WungetL (fun s => θunL (k s))
+      | ImpSet s k => WunsetL s (θunL k)
       | ImpDoWhile body k =>
-        let loop (wcont : Wun bool) : Wun bool := @bind Wun _ _ (θun body) (fun b => if b then wcont else @ret Wun bool false) in
-            (@bind Wun _ _ (ffixun loop) (fun _ => (θun k)))
+        let loop (wcont : Wun bool) : Wun bool := @bind Wun _ _ (θunL body) (fun b => if b then wcont else @ret Wun bool false) in
+            (@bind Wun _ _ (ffixun loop) (fun _ => (θunL k)))
       end.
 
-  Program Definition θun_mm : MonadMorphism Imp_monad Wun := @mkMorphism Imp_monad _ θun _ _.
+  Fixpoint θunR (A : Type) (c: Imp A) {struct c} : Wun A :=
+      match c with
+      | ImpRet a => @ret Wun _ a
+      | ImpGet k => WungetR (fun s => θunR (k s))
+      | ImpSet s k => WunsetR s (θunR k)
+      | ImpDoWhile body k =>
+        let loop (wcont : Wun bool) : Wun bool := @bind Wun _ _ (θunR body) (fun b => if b then wcont else @ret Wun bool false) in
+            (@bind Wun _ _ (ffixun loop) (fun _ => (θunR k)))
+      end.
+
+  Program Definition θunL_mm : MonadMorphism Imp_monad Wun := @mkMorphism Imp_monad _ θunL _ _.
+  Next Obligation.
+    move: m.
+    refine (fix IH (m: Imp A) {struct m} := _).
+    case:m => //= [?|? ?|? ?] ;unfold MonoCont_bind ; apply Ssig_eq; extensionality k=> /=; extensionality s0; rewrite IH //.
+  Qed.
+
+  Program Definition θunR_mm : MonadMorphism Imp_monad Wun := @mkMorphism Imp_monad _ θunR _ _.
   Next Obligation.
     move: m.
     refine (fix IH (m: Imp A) {struct m} := _).
@@ -104,7 +128,54 @@ Section ImpMonad.
   Let M1 := Imp_monad.
   Let M2 := Imp_monad.
 
-  Program Definition θrel := commute_effObs Wun M1 M2 θun_mm θun_mm _.
-  Next Obligation. admit. Admitted.
+  Program Definition θrel := commute_effObs Wun M1 M2 θunL_mm θunR_mm _.
+  Next Obligation. admit.
+    (* move: c1 c2. *)
+    (* refine (fix IH1 (c1: Imp A1) {struct c1} := _). *)
+    (* refine (fix IH2 (c2: Imp A2) {struct c2} := _). *)
+    (* case c1; case c2. *)
+    (* - cbv; intuition. *)
+    (* - cbv; intuition. *)
+    (* - cbv; intuition. *)
+    (* - cbv; intuition. *)
+    (* - cbv; intuition. *)
+    (* - intros i i0. *)
+    (*   unfold commute. simpl. unfold MonoCont_bind. simpl. *)
+  Admitted.
+
+  Notation "⊨ c1 ≈ c2 [{ w }]" := (semantic_judgement _ _ _ θrel _ _ c1 c2 w).
+
+  Definition omega_seq (A : ordType) := nat -> dfst A.
+
+  Definition omega_chain (A : ordType) := { c : omega_seq A ≫ forall (n : nat), c n ≤ c (n + 1) }.
+
+  Definition upper_seq (A : ordType) (c : omega_seq A) (v : dfst A) : SProp :=
+    s∀ n, c n ≤ v.
+
+  Definition sup_seq (A : ordType) (c : omega_seq A) (v : dfst A) : SProp :=
+    upper_seq c v s/\ s∀ v', upper_seq c v' -> v ≤ v'.
+
+  Definition apply_seq (A B : ordType) (c : omega_seq A) (f : dfst A -> dfst B) : omega_seq B := fun n => f (c n).
+
+
+  Definition omega_continuous {A : ordType} (f : dfst A -> dfst A) :=
+    s∀ (c : omega_chain A) v, sup_seq (Spr1 c) v -> sup_seq (apply_seq _ (Spr1 c) f) (f v).
+
+
+  Definition loop (w0 : Wun bool) (wcont : Wun bool) : Wun bool := @bind Wun _ _ w0 (fun b => if b then wcont else @ret Wun bool false).
+
+  Definition preorder_from_type (A : Type) : {R : srelation (Wun A) ≫ PreOrder R}.
+    econstructor.
+    apply (omon_order Wun A).
+  Defined.
+  Definition ordertype_from_type (A : Type) : ordType.
+    econstructor.
+    apply (preorder_from_type A).
+  Defined.
+
+  Program Definition bottom_Wun_seq {A : Type} : omega_chain (ordertype_from_type A) := ⦑fun n =>⦑ fun post s0 => sEmpty ⦒ ⦒.
+  Next Obligation. cbv; intuition. Qed.
+  Next Obligation. sreflexivity. Qed.
+
 
 End ImpMonad.
